killing admits of basic generic actions in HeapSig

pulse/lib/pulse/core/PulseCore.HeapSig.fst
@@ -35,3 +35,176 @@ let cm_slprop (hs:heap_sig u#h)
         hs.star_associative hs.star_commutative
 
 let cm_e_slprop (hs:heap_sig u#h) = erase_cm (cm_slprop hs)
+
+let ac_lemmas (h:heap_sig u#a)
+: Lemma (
+    (forall p q r. (p `h.star` q) `h.star` r == p `h.star` (q `h.star` r)) /\
+    (forall p q. p `h.star` q == q `h.star` p) /\
+    (forall p. p `h.star` h.emp == p)
+)
+= FStar.Classical.forall_intro_3 h.star_associative;
+  FStar.Classical.forall_intro_2 h.star_commutative;
+  FStar.Classical.forall_intro h.emp_unit
+
+let frame
+      (#h:heap_sig u#h)
+      (#opened_invariants:inames h)
+      (#maybe_ghost:bool)
+      (#a:Type u#a)
+      (#pre:h.slprop)
+      (#post:a -> GTot h.slprop)
+      (frame:h.slprop)
+      ($f:_action_except h a maybe_ghost opened_invariants pre post)
+: _action_except h a maybe_ghost opened_invariants (pre `h.star` frame) (fun x -> post x `h.star` frame)
+= fun frame' m -> ac_lemmas h; f (frame `h.star` frame') m
+
+let witness_exists_lemma (#h:heap_sig u#h) (#a:Type u#a)
+             (p:a -> GTot h.slprop) (frame:h.slprop) (m:h.mem { interpret (exists_ p `h.star` frame) m })
+: x:erased a { interpret (p x `h.star` frame) m }
+= h.star_equiv (exists_ p) frame (core_of m);
+  eliminate exists c0 c1.
+    h.sep.disjoint c0 c1 /\
+    core_of m == h.sep.join c0 c1 /\
+    h.interp (exists_ p) c0 /\
+    h.interp frame c1
+  returns (exists (x:a). interpret (p x `h.star` frame) m)
+  with _ . (
+    interp_exists p;
+    eliminate exists x.
+        h.interp (p x) c0
+    returns _
+    with _ . (
+        h.star_equiv (p x) frame (core_of m)
+    )
+  );
+  FStar.IndefiniteDescription.indefinite_description_tot a (fun x -> interpret (p x `h.star` frame) m)
+
+let witness_exists 
+      (#h:heap_sig u#h)
+      (#ex:inames h)
+      (#a:Type u#a)
+      (p:a -> GTot h.slprop)
+: ghost_action_except h (erased a) ex
+           (exists_ p)
+           (fun x -> p x)
+= fun frame m ->
+    ac_lemmas h;
+    let x = witness_exists_lemma p (frame `h.star` h.mem_invariant ex m) m in
+    h.is_ghost_action_preorder ();
+    x, m
+
+let intro_exists_lemma
+      (#h:heap_sig u#h) (#a:Type u#a)
+      (p:a -> GTot h.slprop)
+      (x:erased a)
+      (frame:h.slprop)
+      (m:h.mem { interpret (p x `h.star` frame) m })
+: Lemma (interpret (exists_ p `h.star` frame) m)
+= h.star_equiv (p x) frame (core_of m);
+  interp_exists p;
+  h.star_equiv (exists_ p) frame (core_of m)
+
+let intro_exists
+      (#h:heap_sig u#h)
+      (#opened_invariants:_)
+      (#a:Type u#a)
+      (p:a -> GTot h.slprop)
+      (x:erased a)
+: ghost_action_except h unit opened_invariants
+      (p x)
+      (fun _ -> exists_ p)
+= fun frame m ->
+    ac_lemmas h;
+    intro_exists_lemma p x (frame `h.star` h.mem_invariant opened_invariants m) m;
+    h.is_ghost_action_preorder ();
+    (), m
+
+
+module U = FStar.Universe
+let lift_h_exists
+      (#h:heap_sig u#h)
+      (#opened_invariants:_)
+      (#a:Type u#a)
+      (p:a -> GTot h.slprop)
+: ghost_action_except h unit opened_invariants
+    (exists_ p)
+    (fun _a -> exists_ #_ #(U.raise_t a) (lift_dom_ghost p))
+= fun frame m ->
+    ac_lemmas h;
+    let x = witness_exists_lemma p (frame `h.star` h.mem_invariant opened_invariants m) m in
+    intro_exists_lemma (lift_dom_ghost p) (U.raise_val (reveal x)) (frame `h.star` h.mem_invariant opened_invariants m) m;
+    h.is_ghost_action_preorder ();
+    (), m
+
+
+let emp_trivial (h:heap_sig u#a)
+: Lemma (forall m. h.interp h.emp m)
+= h.pure_true_emp ();
+  FStar.Classical.forall_intro (h.pure_interp True)
+
+let elim_pure_lemma (#h:heap_sig u#h) (p:prop) (frame:h.slprop) 
+    (m:h.mem { interpret (h.pure p `h.star` frame) m })
+: Lemma (p /\ interpret (h.emp `h.star` frame) m)
+= h.star_equiv (h.pure p) frame (core_of m);
+  FStar.Classical.forall_intro (h.pure_interp p);
+  h.star_equiv h.emp frame (core_of m);
+  emp_trivial h
+
+let elim_pure
+      (#h:heap_sig u#h)
+      (#opened_invariants:_)
+      (p:prop)
+: ghost_action_except h (squash p) opened_invariants (h.pure p) (fun _ -> h.emp)
+= fun frame m ->
+    ac_lemmas h;
+    elim_pure_lemma p (frame `h.star` h.mem_invariant opened_invariants m) m;
+    h.is_ghost_action_preorder ();
+    (), m
+
+let intro_pure_lemma (#h:heap_sig u#h) (p:prop) (frame:h.slprop) (pf:squash p)
+    (m:h.mem { interpret (h.emp `h.star` frame) m })
+: Lemma (interpret (h.pure p `h.star` frame) m)
+= h.star_equiv h.emp frame (core_of m);
+  FStar.Classical.forall_intro (h.pure_interp p);
+  h.star_equiv (h.pure p) frame (core_of m)
+
+let intro_pure
+      (#h:heap_sig u#h)
+      (#opened_invariants:_)
+      (p:prop)
+      (pf:squash p)
+: ghost_action_except h unit opened_invariants h.emp (fun _ -> h.pure p)
+= fun frame m ->
+    ac_lemmas h;
+    intro_pure_lemma p (frame `h.star` h.mem_invariant opened_invariants m) pf m;
+    h.is_ghost_action_preorder ();
+    (), m
+
+let drop_lemma (#h:heap_sig u#h) (p:h.slprop) (frame:h.slprop)
+    (m:h.mem { interpret (p `h.star` frame) m })
+: Lemma (interpret (h.emp `h.star` frame) m)
+= emp_trivial h;
+  h.star_equiv p frame (core_of m);
+  h.star_equiv h.emp frame (core_of m)
+
+let drop 
+      (#h:heap_sig u#h)
+      (#opened_invariants:_)
+      (p:h.slprop)
+: ghost_action_except h unit opened_invariants p (fun _ -> h.emp)
+= fun frame m ->
+    ac_lemmas h;
+    drop_lemma p (frame `h.star` h.mem_invariant opened_invariants m) m;
+    h.is_ghost_action_preorder ();
+    (), m
+
+let lift_ghost
+      (#h:heap_sig u#h)
+      (#opened_invariants:inames h)
+      (#a:Type u#a)
+      (#p:h.slprop)
+      (#q:a -> GTot h.slprop)
+      (ni_a:non_info a)
+      (f:erased (ghost_action_except h a opened_invariants p q))
+: ghost_action_except h a opened_invariants p q
+= admit()
